Pullback/UnquoteTy/Do.lean
@@ -1,0 +1,50 @@
+import Pullback.UnquoteTy.Basic
+/-! # Basic `do` notation -/
+
+open Lean
+
+declare_syntax_cat stmt
+syntax "do'" stmt : term
+
+-- Prevent `if ...` from being parsed as a term
+syntax (priority := low) term : stmt
+syntax "let" ident "←" stmt:1 ";" stmt : stmt
+macro "{" s:stmt "}" : stmt => `(stmt| $s)
+
+/-
+  Remark: we annotate `macro`s and `macro_rules` with their corresponding
+  translation/abbreviation id from the paper.
+-/
+
+syntax "d!" stmt : term  -- corresponds to `D(s)`
+
+macro_rules
+  | `(do' $s) => `(d! $s)  -- (1)
+
+-- helper function; see usage below
+def expandStmt (s : TSyntax `stmt) : MacroM (TSyntax `stmt) := do
+  let s' ← expandMacros s
+  if s == s' then
+    Macro.throwUnsupported
+  else
+    -- There is no static guarantee that `expandMacros` stays in the `stmt` category,
+    -- but it is true for all our macros
+    return TSyntax.mk s'
+
+#check UnquoteTy.app
+macro_rules
+  | `(d! $e:term) => `($e)                                       -- (D1)
+  | `(d! let $x ← $s; $s') => `(UnquoteTy.app (UnquoteTy.app MonadTy.bind (d! $s)) (fun $x => (d! $s')))  -- (D2)
+  | `(d! $s) => do
+    -- fallback rule: try to expand abbreviation
+    let s' ← expandStmt s
+    `(d! $s')
+
+macro "let" x:ident ":=" e:term ";" s:stmt : stmt => `(stmt| let $x ← MonadTy.pure $e; $s)  -- (A1)
+-- priority `0` prevents `;` from being used in trailing contexts without braces (see e.g. `:1` above)
+macro:0 s₁:stmt ";" s₂:stmt : stmt => `(stmt| let x ← $s₁; $s₂)                     -- (A2)
+
+open UnquoteTy MonadTy
+def test : «syntax» (id SimpleTy.nat) := do'
+  let x := 10;
+  return x
